src/Coinductive_Prop.thy
@@ -21,6 +21,8 @@ fun TESL_interpretation_primitive_at_index
                          \<and> time ((Rep_run \<rho>) n K\<^sub>2) = time ((Rep_run \<rho>) n\<^sub>p\<^sub>a\<^sub>s\<^sub>t K\<^sub>p\<^sub>a\<^sub>s\<^sub>t) + \<delta>\<tau> }"
   | "\<lbrakk> tag-relation K\<^sub>1 = \<alpha> * K\<^sub>2 + \<beta> \<rbrakk>\<^sub>T\<^sub>E\<^sub>S\<^sub>L\<^bsup>\<ge> i\<^esup> =
         { \<rho>. \<forall>n\<ge>i. time ((Rep_run \<rho>) n K\<^sub>1) = \<alpha> * time ((Rep_run \<rho>) n K\<^sub>2) + \<beta> }"
+  | "\<lbrakk> tag-relation \<langle>K\<^sub>1, K\<^sub>2\<rangle> \<in> R \<rbrakk>\<^sub>T\<^sub>E\<^sub>S\<^sub>L\<^bsup>\<ge> i\<^esup> =
+        { \<rho>. \<forall>n\<ge>i. R (time ((Rep_run \<rho>) n K\<^sub>1), time ((Rep_run \<rho>) n K\<^sub>2)) }"
   | "\<lbrakk> master implies slave \<rbrakk>\<^sub>T\<^sub>E\<^sub>S\<^sub>L\<^bsup>\<ge> i\<^esup> =
         { \<rho>. \<forall>n\<ge>i. hamlet ((Rep_run \<rho>) n master) \<longrightarrow> hamlet ((Rep_run \<rho>) n slave) }"
   | "\<lbrakk> master time-delayed by \<delta>\<tau> on measuring implies slave \<rbrakk>\<^sub>T\<^sub>E\<^sub>S\<^sub>L\<^bsup>\<ge> i\<^esup> =
@@ -55,6 +57,10 @@ lemma TESL_interp_unfold_at_index_tagrel:
   shows "\<lbrakk> tag-relation K\<^sub>1 = \<alpha> * K\<^sub>2 + \<beta> \<rbrakk>\<^sub>T\<^sub>E\<^sub>S\<^sub>L = \<Inter> {Y. \<exists>n::nat. Y = \<lbrakk> tag-relation K\<^sub>1 = \<alpha> * K\<^sub>2 + \<beta> \<rbrakk>\<^sub>T\<^sub>E\<^sub>S\<^sub>L\<^bsup>\<ge> n\<^esup>}"
   by auto
 
+lemma TESL_interp_unfold_at_index_tagrelgen:
+  shows "\<lbrakk> tag-relation \<langle>K\<^sub>1, K\<^sub>2\<rangle> \<in> R \<rbrakk>\<^sub>T\<^sub>E\<^sub>S\<^sub>L = \<Inter> {Y. \<exists>n::nat. Y = \<lbrakk> tag-relation \<langle>K\<^sub>1, K\<^sub>2\<rangle> \<in> R \<rbrakk>\<^sub>T\<^sub>E\<^sub>S\<^sub>L\<^bsup>\<ge> n\<^esup>}"
+  by auto
+
 lemma TESL_interp_unfold_at_index_implies:
   shows "\<lbrakk> master implies slave \<rbrakk>\<^sub>T\<^sub>E\<^sub>S\<^sub>L = \<Inter> {Y. \<exists>n::nat. Y = \<lbrakk> master implies slave \<rbrakk>\<^sub>T\<^sub>E\<^sub>S\<^sub>L\<^bsup>\<ge> n\<^esup>}"
   by auto
@@ -83,7 +89,7 @@ theorem TESL_interp_unfold_at_index_positive_atoms:
 theorem TESL_interp_unfold_at_index_negative_atoms:
   assumes "\<not> positive_atom \<phi>"
   shows "\<lbrakk> \<phi> \<rbrakk>\<^sub>T\<^sub>E\<^sub>S\<^sub>L = \<Inter> {Y. \<exists>n::nat. Y = \<lbrakk> \<phi> \<rbrakk>\<^sub>T\<^sub>E\<^sub>S\<^sub>L\<^bsup>\<ge> n\<^esup>}"
-  by (smt Collect_cong TESL_interp_unfold_at_index_implies TESL_interp_unfold_at_index_tagrel TESL_interp_unfold_at_index_timedelayed assms positive_atom.elims(3))
+  by (smt Collect_cong TESL_interp_unfold_at_index_implies TESL_interp_unfold_at_index_tagrel TESL_interp_unfold_at_index_tagrelgen TESL_interp_unfold_at_index_timedelayed assms positive_atom.elims(3))
 
 lemma forall_nat_expansion:
   "(\<forall>n\<^sub>1 \<ge> (n\<^sub>0::nat). P n\<^sub>1) \<equiv> P n\<^sub>0 \<and> (\<forall>n\<^sub>1 \<ge> Suc n\<^sub>0. P n\<^sub>1)"
@@ -169,6 +175,18 @@ lemma TESL_interp_at_index_tagrel_cases:
   then show ?thesis by auto
   qed
 
+lemma TESL_interp_at_index_tagrelgen_cases:
+  shows "\<lbrakk> tag-relation \<langle>K\<^sub>1, K\<^sub>2\<rangle> \<in> R \<rbrakk>\<^sub>T\<^sub>E\<^sub>S\<^sub>L\<^bsup>\<ge> n\<^esup> =
+    \<lbrakk> \<langle>\<tau>\<^sub>v\<^sub>a\<^sub>r(K\<^sub>1, n), \<tau>\<^sub>v\<^sub>a\<^sub>r(K\<^sub>2, n)\<rangle> \<epsilon> R \<rbrakk>\<^sub>s\<^sub>y\<^sub>m\<^sub>r\<^sub>u\<^sub>n
+    \<inter> \<lbrakk> tag-relation \<langle>K\<^sub>1, K\<^sub>2\<rangle> \<in> R \<rbrakk>\<^sub>T\<^sub>E\<^sub>S\<^sub>L\<^bsup>\<ge> Suc n\<^esup>"
+  proof -
+    have "{ \<rho>. \<forall>m\<ge>n. R (time ((Rep_run \<rho>) m K\<^sub>1), time ((Rep_run \<rho>) m K\<^sub>2)) }
+         = { \<rho>. R (time ((Rep_run \<rho>) n K\<^sub>1), time ((Rep_run \<rho>) n K\<^sub>2)) }
+         \<inter> { \<rho>. \<forall>m\<ge>Suc n. R (time ((Rep_run \<rho>) m K\<^sub>1), time ((Rep_run \<rho>) m K\<^sub>2)) }"
+      by (smt Collect_cong Collect_conj_eq Suc_leD eq_refl le_antisym not_less_eq_eq)
+  then show ?thesis by auto
+  qed
+
 lemma TESL_interp_at_index_implies_cases:
   shows "\<lbrakk> master implies slave \<rbrakk>\<^sub>T\<^sub>E\<^sub>S\<^sub>L\<^bsup>\<ge> n\<^esup> =
     (\<lbrakk> master \<not>\<Up> n \<rbrakk>\<^sub>s\<^sub>y\<^sub>m\<^sub>r\<^sub>u\<^sub>n \<union> \<lbrakk> master \<Up> n \<rbrakk>\<^sub>s\<^sub>y\<^sub>m\<^sub>r\<^sub>u\<^sub>n \<inter> \<lbrakk> slave \<Up> n \<rbrakk>\<^sub>s\<^sub>y\<^sub>m\<^sub>r\<^sub>u\<^sub>n)
@@ -238,6 +256,9 @@ lemma TESL_interpretation_at_index_zero:
       qed
   next
     case (TagRelation x1 x2 x3 x4)
+    then show ?case by simp
+  next
+    case (TagRelationGen x1 x2 x3)
     then show ?case by simp
   next
     case (Implies x1 x2)
@@ -353,6 +374,24 @@ lemma HeronConf_interp_at_index_tagrel_cases:
     proof -
       have "\<lbrakk> \<tau>\<^sub>v\<^sub>a\<^sub>r (K\<^sub>1, n) \<doteq> \<alpha> * \<tau>\<^sub>v\<^sub>a\<^sub>r (K\<^sub>2, n) + \<beta> \<rbrakk>\<^sub>s\<^sub>y\<^sub>m\<^sub>r\<^sub>u\<^sub>n \<inter> \<lbrakk> tag-relation K\<^sub>1 = \<alpha> * K\<^sub>2 + \<beta> \<rbrakk>\<^sub>T\<^sub>E\<^sub>S\<^sub>L\<^bsup>\<ge> Suc n\<^esup> \<inter> \<lbrakk>\<lbrakk> \<Psi> \<rbrakk>\<rbrakk>\<^sub>T\<^sub>E\<^sub>S\<^sub>L\<^bsup>\<ge> n\<^esup> = \<lbrakk>\<lbrakk> (tag-relation K\<^sub>1 = \<alpha> * K\<^sub>2 + \<beta>) # \<Psi> \<rbrakk>\<rbrakk>\<^sub>T\<^sub>E\<^sub>S\<^sub>L\<^bsup>\<ge> n\<^esup>"
         using TESL_interp_at_index_tagrel_cases TESL_interpretation_at_index_cons_morph by blast
+      then show ?thesis
+        by auto
+    qed
+  qed
+
+lemma HeronConf_interp_at_index_tagrelgen_cases:
+  shows "\<lbrakk> \<Gamma>, n \<turnstile> (tag-relation \<langle>K\<^sub>1, K\<^sub>2\<rangle> \<in> R) # \<Psi> \<triangleright> \<Phi> \<rbrakk>\<^sub>c\<^sub>o\<^sub>n\<^sub>f\<^sub>i\<^sub>g
+          = \<lbrakk> (\<langle>\<tau>\<^sub>v\<^sub>a\<^sub>r(K\<^sub>1, n), \<tau>\<^sub>v\<^sub>a\<^sub>r(K\<^sub>2, n)\<rangle> \<epsilon> R) # \<Gamma>, n \<turnstile> \<Psi> \<triangleright> (tag-relation \<langle>K\<^sub>1, K\<^sub>2\<rangle> \<in> R) # \<Phi> \<rbrakk>\<^sub>c\<^sub>o\<^sub>n\<^sub>f\<^sub>i\<^sub>g"
+  proof -
+    have "\<lbrakk> \<Gamma>, n \<turnstile> (tag-relation \<langle>K\<^sub>1, K\<^sub>2\<rangle> \<in> R) # \<Psi> \<triangleright> \<Phi> \<rbrakk>\<^sub>c\<^sub>o\<^sub>n\<^sub>f\<^sub>i\<^sub>g = \<lbrakk>\<lbrakk> \<Gamma> \<rbrakk>\<rbrakk>\<^sub>s\<^sub>y\<^sub>m\<^sub>r\<^sub>u\<^sub>n \<inter> \<lbrakk>\<lbrakk> (tag-relation \<langle>K\<^sub>1, K\<^sub>2\<rangle> \<in> R) # \<Psi> \<rbrakk>\<rbrakk>\<^sub>T\<^sub>E\<^sub>S\<^sub>L\<^bsup>\<ge> n\<^esup> \<inter> \<lbrakk>\<lbrakk> \<Phi> \<rbrakk>\<rbrakk>\<^sub>T\<^sub>E\<^sub>S\<^sub>L\<^bsup>\<ge> Suc n\<^esup>"
+      by simp
+    moreover have "\<lbrakk> (\<langle>\<tau>\<^sub>v\<^sub>a\<^sub>r(K\<^sub>1, n), \<tau>\<^sub>v\<^sub>a\<^sub>r(K\<^sub>2, n)\<rangle> \<epsilon> R) # \<Gamma>, n \<turnstile> \<Psi> \<triangleright> (tag-relation \<langle>K\<^sub>1, K\<^sub>2\<rangle> \<in> R) # \<Phi> \<rbrakk>\<^sub>c\<^sub>o\<^sub>n\<^sub>f\<^sub>i\<^sub>g
+                      = \<lbrakk>\<lbrakk> (\<langle>\<tau>\<^sub>v\<^sub>a\<^sub>r(K\<^sub>1, n), \<tau>\<^sub>v\<^sub>a\<^sub>r(K\<^sub>2, n)\<rangle> \<epsilon> R) # \<Gamma> \<rbrakk>\<rbrakk>\<^sub>s\<^sub>y\<^sub>m\<^sub>r\<^sub>u\<^sub>n \<inter> \<lbrakk>\<lbrakk> \<Psi> \<rbrakk>\<rbrakk>\<^sub>T\<^sub>E\<^sub>S\<^sub>L\<^bsup>\<ge> n\<^esup> \<inter> \<lbrakk>\<lbrakk> (tag-relation \<langle>K\<^sub>1, K\<^sub>2\<rangle> \<in> R) # \<Phi> \<rbrakk>\<rbrakk>\<^sub>T\<^sub>E\<^sub>S\<^sub>L\<^bsup>\<ge> Suc n\<^esup>"
+      by simp
+    ultimately show ?thesis
+    proof -
+      have "\<lbrakk> \<langle>\<tau>\<^sub>v\<^sub>a\<^sub>r(K\<^sub>1, n), \<tau>\<^sub>v\<^sub>a\<^sub>r(K\<^sub>2, n)\<rangle> \<epsilon> R \<rbrakk>\<^sub>s\<^sub>y\<^sub>m\<^sub>r\<^sub>u\<^sub>n \<inter> \<lbrakk> tag-relation \<langle>K\<^sub>1, K\<^sub>2\<rangle> \<in> R \<rbrakk>\<^sub>T\<^sub>E\<^sub>S\<^sub>L\<^bsup>\<ge> Suc n\<^esup> \<inter> \<lbrakk>\<lbrakk> \<Psi> \<rbrakk>\<rbrakk>\<^sub>T\<^sub>E\<^sub>S\<^sub>L\<^bsup>\<ge> n\<^esup> = \<lbrakk>\<lbrakk> (tag-relation \<langle>K\<^sub>1, K\<^sub>2\<rangle> \<in> R) # \<Psi> \<rbrakk>\<rbrakk>\<^sub>T\<^sub>E\<^sub>S\<^sub>L\<^bsup>\<ge> n\<^esup>"
+        using TESL_interp_at_index_tagrelgen_cases TESL_interpretation_at_index_cons_morph by blast
       then show ?thesis
         by auto
     qed
