src/Denotational.thy
@@ -19,6 +19,8 @@ fun TESL_interpretation_atomic
                        \<and> time ((Rep_run \<rho>) n K\<^sub>2) = time ((Rep_run \<rho>) n\<^sub>i K\<^sub>i) + \<delta>\<tau> }"
   | "\<lbrakk> tag-relation K\<^sub>1 = \<alpha> * K\<^sub>2 + \<beta> \<rbrakk>\<^sub>T\<^sub>E\<^sub>S\<^sub>L =
         { \<rho>. \<forall>n::nat. time ((Rep_run \<rho>) n K\<^sub>1) = \<alpha> * time ((Rep_run \<rho>) n K\<^sub>2) + \<beta> }"
+  | "\<lbrakk> tag-relation \<langle>K\<^sub>1, K\<^sub>2\<rangle> \<in> R \<rbrakk>\<^sub>T\<^sub>E\<^sub>S\<^sub>L =
+        { \<rho>. \<forall>n::nat. R (time ((Rep_run \<rho>) n K\<^sub>1), time ((Rep_run \<rho>) n K\<^sub>2)) }"
   | "\<lbrakk> master implies slave \<rbrakk>\<^sub>T\<^sub>E\<^sub>S\<^sub>L =
         { \<rho>. \<forall>n::nat. hamlet ((Rep_run \<rho>) n master) \<longrightarrow> hamlet ((Rep_run \<rho>) n slave) }"
   | "\<lbrakk> master time-delayed by \<delta>\<tau> on measuring implies slave \<rbrakk>\<^sub>T\<^sub>E\<^sub>S\<^sub>L =
