src/Hygge_Theory.thy
@@ -80,6 +80,14 @@ lemma reduction_step_sound:
        \<lbrakk>\<lbrakk> \<Gamma>\<^sub>2 \<rbrakk>\<rbrakk>\<^sub>s\<^sub>y\<^sub>m\<^sub>r\<^sub>u\<^sub>n \<inter> \<lbrakk>\<lbrakk> \<Psi>\<^sub>2 \<rbrakk>\<rbrakk>\<^sub>T\<^sub>E\<^sub>S\<^sub>L\<^bsup>\<ge> n\<^sub>2\<^esup> \<inter> \<lbrakk>\<lbrakk> \<Phi>\<^sub>2 \<rbrakk>\<rbrakk>\<^sub>T\<^sub>E\<^sub>S\<^sub>L\<^bsup>\<ge> Suc n\<^sub>2\<^esup>
        \<subseteq> \<lbrakk>\<lbrakk> \<Gamma>\<^sub>1 \<rbrakk>\<rbrakk>\<^sub>s\<^sub>y\<^sub>m\<^sub>r\<^sub>u\<^sub>n \<inter> \<lbrakk>\<lbrakk> \<Psi>\<^sub>1 \<rbrakk>\<rbrakk>\<^sub>T\<^sub>E\<^sub>S\<^sub>L\<^bsup>\<ge> n\<^sub>1\<^esup> \<inter> \<lbrakk>\<lbrakk> \<Phi>\<^sub>1 \<rbrakk>\<rbrakk>\<^sub>T\<^sub>E\<^sub>S\<^sub>L\<^bsup>\<ge> Suc n\<^sub>1\<^esup>"
       using HeronConf_interp_at_index_tagrel_cases by auto
+    show "\<And>\<Gamma>\<^sub>1' n\<^sub>1' \<Psi>\<^sub>1' \<Phi>\<^sub>1' \<Gamma>\<^sub>2' n\<^sub>2' \<Psi>\<^sub>2' \<Phi>\<^sub>2' \<Gamma> n K\<^sub>1 K\<^sub>2 R \<Psi> \<Phi>.
+       (\<Gamma>\<^sub>1, n\<^sub>1 \<turnstile> \<Psi>\<^sub>1 \<triangleright> \<Phi>\<^sub>1) = \<Gamma>\<^sub>1', n\<^sub>1' \<turnstile> \<Psi>\<^sub>1' \<triangleright> \<Phi>\<^sub>1' \<Longrightarrow>
+       (\<Gamma>\<^sub>2, n\<^sub>2 \<turnstile> \<Psi>\<^sub>2 \<triangleright> \<Phi>\<^sub>2) = \<Gamma>\<^sub>2', n\<^sub>2' \<turnstile> \<Psi>\<^sub>2' \<triangleright> \<Phi>\<^sub>2' \<Longrightarrow>
+       (\<Gamma>\<^sub>1', n\<^sub>1' \<turnstile> \<Psi>\<^sub>1' \<triangleright> \<Phi>\<^sub>1') = \<Gamma>, n \<turnstile> (tag-relation \<langle>K\<^sub>1, K\<^sub>2\<rangle> \<in> R) # \<Psi> \<triangleright> \<Phi> \<Longrightarrow>
+       (\<Gamma>\<^sub>2', n\<^sub>2' \<turnstile> \<Psi>\<^sub>2' \<triangleright> \<Phi>\<^sub>2') = \<langle>\<tau>\<^sub>v\<^sub>a\<^sub>r(K\<^sub>1, n), \<tau>\<^sub>v\<^sub>a\<^sub>r(K\<^sub>2, n)\<rangle> \<epsilon> R # \<Gamma>, n \<turnstile> \<Psi> \<triangleright> (tag-relation \<langle>K\<^sub>1, K\<^sub>2\<rangle> \<in> R) # \<Phi> \<Longrightarrow>
+       \<lbrakk>\<lbrakk> \<Gamma>\<^sub>2 \<rbrakk>\<rbrakk>\<^sub>s\<^sub>y\<^sub>m\<^sub>r\<^sub>u\<^sub>n \<inter> \<lbrakk>\<lbrakk> \<Psi>\<^sub>2 \<rbrakk>\<rbrakk>\<^sub>T\<^sub>E\<^sub>S\<^sub>L\<^bsup>\<ge> n\<^sub>2\<^esup> \<inter> \<lbrakk>\<lbrakk> \<Phi>\<^sub>2 \<rbrakk>\<rbrakk>\<^sub>T\<^sub>E\<^sub>S\<^sub>L\<^bsup>\<ge> Suc n\<^sub>2\<^esup>
+       \<subseteq> \<lbrakk>\<lbrakk> \<Gamma>\<^sub>1 \<rbrakk>\<rbrakk>\<^sub>s\<^sub>y\<^sub>m\<^sub>r\<^sub>u\<^sub>n \<inter> \<lbrakk>\<lbrakk> \<Psi>\<^sub>1 \<rbrakk>\<rbrakk>\<^sub>T\<^sub>E\<^sub>S\<^sub>L\<^bsup>\<ge> n\<^sub>1\<^esup> \<inter> \<lbrakk>\<lbrakk> \<Phi>\<^sub>1 \<rbrakk>\<rbrakk>\<^sub>T\<^sub>E\<^sub>S\<^sub>L\<^bsup>\<ge> Suc n\<^sub>1\<^esup>"
+      using HeronConf_interp_at_index_tagrelgen_cases by auto
     show "\<And>\<Gamma>\<^sub>1' n\<^sub>1' \<Psi>\<^sub>1' \<Phi>\<^sub>1' \<Gamma>\<^sub>2' n\<^sub>2' \<Psi>\<^sub>2' \<Phi>\<^sub>2' \<Gamma> n K\<^sub>1 K\<^sub>2 \<Psi> \<Phi>.
        (\<Gamma>\<^sub>1, n\<^sub>1 \<turnstile> \<Psi>\<^sub>1 \<triangleright> \<Phi>\<^sub>1) = \<Gamma>\<^sub>1', n\<^sub>1' \<turnstile> \<Psi>\<^sub>1' \<triangleright> \<Phi>\<^sub>1' \<Longrightarrow>
        (\<Gamma>\<^sub>2, n\<^sub>2 \<turnstile> \<Psi>\<^sub>2 \<triangleright> \<Phi>\<^sub>2) = \<Gamma>\<^sub>2', n\<^sub>2' \<turnstile> \<Psi>\<^sub>2' \<triangleright> \<Phi>\<^sub>2' \<Longrightarrow>
@@ -186,6 +194,11 @@ lemma coverage_complete:
         case (TagRelation K1 \<alpha> K2 \<beta>)
         then show ?case
           using HeronConf_interp_at_index_tagrel_cases Fnext_solve_tagrel
+          by (smt UN_iff UnE insert_subset subsetI)
+      next
+        case (TagRelationGen K\<^sub>1 K\<^sub>2 R)
+        then show ?case
+          using HeronConf_interp_at_index_tagrelgen_cases Fnext_solve_tagrelgen
           by (smt UN_iff UnE insert_subset subsetI)
       next
         case (Implies K1 K2)
@@ -362,6 +375,19 @@ lemma instant_index_increase:
             by (meson elims_part relpowp_Suc_I2 tagrel_e)
         qed
     next
+      case (TagRelationGen K\<^sub>1 K\<^sub>2 R)
+      have branches: "\<lbrakk> \<Gamma>, k \<turnstile> (tag-relation \<langle>K\<^sub>1, K\<^sub>2\<rangle> \<in> R) # \<Psi> \<triangleright> \<Phi> \<rbrakk>\<^sub>c\<^sub>o\<^sub>n\<^sub>f\<^sub>i\<^sub>g
+          = \<lbrakk> (\<langle>\<tau>\<^sub>v\<^sub>a\<^sub>r(K\<^sub>1, k), \<tau>\<^sub>v\<^sub>a\<^sub>r(K\<^sub>2, k)\<rangle> \<epsilon> R) # \<Gamma>, k \<turnstile> \<Psi> \<triangleright> (tag-relation \<langle>K\<^sub>1, K\<^sub>2\<rangle> \<in> R) # \<Phi> \<rbrakk>\<^sub>c\<^sub>o\<^sub>n\<^sub>f\<^sub>i\<^sub>g"
+        using HeronConf_interp_at_index_tagrelgen_cases by simp
+      then show ?case
+        proof -
+          have "\<exists>\<Gamma>\<^sub>n \<Psi>\<^sub>n \<Phi>\<^sub>n n. ((\<langle>\<tau>\<^sub>v\<^sub>a\<^sub>r(K\<^sub>1, k), \<tau>\<^sub>v\<^sub>a\<^sub>r(K\<^sub>2, k)\<rangle> \<epsilon> R) # \<Gamma>, k \<turnstile> \<Psi> \<triangleright> (tag-relation \<langle>K\<^sub>1, K\<^sub>2\<rangle> \<in> R) # \<Phi>)
+              \<hookrightarrow>\<^bsup>n\<^esup> \<Gamma>\<^sub>n, Suc k \<turnstile> \<Psi>\<^sub>n \<triangleright> \<Phi>\<^sub>n \<and> \<rho> \<in> \<lbrakk> \<Gamma>\<^sub>n, Suc k \<turnstile> \<Psi>\<^sub>n \<triangleright> \<Phi>\<^sub>n \<rbrakk>\<^sub>c\<^sub>o\<^sub>n\<^sub>f\<^sub>i\<^sub>g"
+            using TagRelationGen.prems by simp
+          then show ?thesis
+            by (meson elims_part relpowp_Suc_I2 tagrelgen_e)
+        qed
+    next
       case (Implies K\<^sub>1 K\<^sub>2)
       have branches: "\<lbrakk> \<Gamma>, k \<turnstile> (K\<^sub>1 implies K\<^sub>2) # \<Psi> \<triangleright> \<Phi> \<rbrakk>\<^sub>c\<^sub>o\<^sub>n\<^sub>f\<^sub>i\<^sub>g
           = \<lbrakk> K\<^sub>1 \<not>\<Up> k # \<Gamma>, k \<turnstile> \<Psi> \<triangleright> (K\<^sub>1 implies K\<^sub>2) # \<Phi> \<rbrakk>\<^sub>c\<^sub>o\<^sub>n\<^sub>f\<^sub>i\<^sub>g
@@ -395,8 +421,8 @@ lemma instant_index_increase:
           = \<lbrakk> K\<^sub>1 \<not>\<Up> k # \<Gamma>, k \<turnstile> \<Psi> \<triangleright> (K\<^sub>1 time-delayed by \<delta>\<tau> on K\<^sub>2 implies K\<^sub>3) # \<Phi> \<rbrakk>\<^sub>c\<^sub>o\<^sub>n\<^sub>f\<^sub>i\<^sub>g
           \<union> \<lbrakk> K\<^sub>1 \<Up> k # \<Gamma>, k \<turnstile> (K\<^sub>3 sporadic \<lfloor>\<tau>\<^sub>v\<^sub>a\<^sub>r(K\<^sub>2, k) \<oplus> \<delta>\<tau>\<rfloor> on K\<^sub>2) # \<Psi> \<triangleright> (K\<^sub>1 time-delayed by \<delta>\<tau> on K\<^sub>2 implies K\<^sub>3) # \<Phi> \<rbrakk>\<^sub>c\<^sub>o\<^sub>n\<^sub>f\<^sub>i\<^sub>g"
         using HeronConf_interp_at_index_timedelayed_cases by simp
-      have more_branches: "\<lbrakk> K\<^sub>1 \<Up> k # \<Gamma>, k \<turnstile> (K\<^sub>3 sporadic \<lfloor>\<tau>\<^sub>v\<^sub>a\<^sub>r(K\<^sub>2, k) \<oplus> \<delta>\<tau>\<rfloor> on K\<^sub>2) # \<Psi> \<triangleright> (K\<^sub>1 time-delayed by \<delta>\<tau> on K\<^sub>2 implies K\<^sub>3) # \<Phi> \<rbrakk>\<^sub>c\<^sub>o\<^sub>n\<^sub>f\<^sub>i\<^sub>g
-                  = \<lbrakk> K\<^sub>1 \<Up> k # \<Gamma>, k \<turnstile> \<Psi> \<triangleright> (K\<^sub>3 sporadic \<lfloor>\<tau>\<^sub>v\<^sub>a\<^sub>r(K\<^sub>2, k) \<oplus> \<delta>\<tau>\<rfloor> on K\<^sub>2) # (K\<^sub>1 time-delayed by \<delta>\<tau> on K\<^sub>2 implies K\<^sub>3) # \<Phi> \<rbrakk>\<^sub>c\<^sub>o\<^sub>n\<^sub>f\<^sub>i\<^sub>g
+      have more_branches: "\<lbrakk> (K\<^sub>1 \<Up> k) # \<Gamma>, k \<turnstile> (K\<^sub>3 sporadic \<lfloor>\<tau>\<^sub>v\<^sub>a\<^sub>r(K\<^sub>2, k) \<oplus> \<delta>\<tau>\<rfloor> on K\<^sub>2) # \<Psi> \<triangleright> (K\<^sub>1 time-delayed by \<delta>\<tau> on K\<^sub>2 implies K\<^sub>3) # \<Phi> \<rbrakk>\<^sub>c\<^sub>o\<^sub>n\<^sub>f\<^sub>i\<^sub>g
+                  = \<lbrakk> (K\<^sub>1 \<Up> k) # \<Gamma>, k \<turnstile> \<Psi> \<triangleright> (K\<^sub>3 sporadic \<lfloor>\<tau>\<^sub>v\<^sub>a\<^sub>r(K\<^sub>2, k) \<oplus> \<delta>\<tau>\<rfloor> on K\<^sub>2) # (K\<^sub>1 time-delayed by \<delta>\<tau> on K\<^sub>2 implies K\<^sub>3) # \<Phi> \<rbrakk>\<^sub>c\<^sub>o\<^sub>n\<^sub>f\<^sub>i\<^sub>g
                   \<union> \<lbrakk> (K\<^sub>3 \<Up> k) # (K\<^sub>2 \<Down> k @ \<lfloor>\<tau>\<^sub>v\<^sub>a\<^sub>r(K\<^sub>2, k) \<oplus> \<delta>\<tau>\<rfloor>) # (K\<^sub>1 \<Up> k) # \<Gamma>, k \<turnstile> \<Psi> \<triangleright> (K\<^sub>1 time-delayed by \<delta>\<tau> on K\<^sub>2 implies K\<^sub>3) # \<Phi> \<rbrakk>\<^sub>c\<^sub>o\<^sub>n\<^sub>f\<^sub>i\<^sub>g"
             using HeronConf_interp_at_index_sporadicon_cases by blast
       have br1: "\<rho> \<in> \<lbrakk> K\<^sub>1 \<not>\<Up> k # \<Gamma>, k \<turnstile> \<Psi> \<triangleright> (K\<^sub>1 time-delayed by \<delta>\<tau> on K\<^sub>2 implies K\<^sub>3) # \<Phi> \<rbrakk>\<^sub>c\<^sub>o\<^sub>n\<^sub>f\<^sub>i\<^sub>g \<Longrightarrow> \<exists>\<Gamma>\<^sub>n \<Psi>\<^sub>n \<Phi>\<^sub>n n.
