src/Run.thy
@@ -36,6 +36,7 @@ fun symbolic_run_interpretation_primitive :: "constr \<Rightarrow> run set" ("\<
   | "\<lbrakk> K \<Down> n @ \<lfloor> \<tau> \<rfloor> \<rbrakk>\<^sub>s\<^sub>y\<^sub>m\<^sub>r\<^sub>u\<^sub>n = { \<rho>. time ((Rep_run \<rho>) n K) = \<tau> }"
   | "\<lbrakk> K \<Down> n @ \<lfloor> \<tau>\<^sub>v\<^sub>a\<^sub>r(K', n') \<oplus> \<tau> \<rfloor> \<rbrakk>\<^sub>s\<^sub>y\<^sub>m\<^sub>r\<^sub>u\<^sub>n = { \<rho>. time ((Rep_run \<rho>) n K) = time ((Rep_run \<rho>) n' K') + \<tau> }"
   | "\<lbrakk> \<tau>\<^sub>v\<^sub>a\<^sub>r(K\<^sub>1, n\<^sub>1) \<doteq> \<alpha> * \<tau>\<^sub>v\<^sub>a\<^sub>r(K\<^sub>2, n\<^sub>2) + \<beta> \<rbrakk>\<^sub>s\<^sub>y\<^sub>m\<^sub>r\<^sub>u\<^sub>n = { \<rho>. time ((Rep_run \<rho>) n\<^sub>1 K\<^sub>1) = \<alpha> * time ((Rep_run \<rho>) n\<^sub>2 K\<^sub>2) + \<beta> }"
+  | "\<lbrakk> \<langle>\<tau>\<^sub>v\<^sub>a\<^sub>r(K\<^sub>1, n\<^sub>1), \<tau>\<^sub>v\<^sub>a\<^sub>r(K\<^sub>2, n\<^sub>2)\<rangle> \<epsilon> R \<rbrakk>\<^sub>s\<^sub>y\<^sub>m\<^sub>r\<^sub>u\<^sub>n = { \<rho>. R (time ((Rep_run \<rho>) n\<^sub>1 K\<^sub>1), time ((Rep_run \<rho>) n\<^sub>2 K\<^sub>2)) }"
 
 fun symbolic_run_interpretation :: "constr list \<Rightarrow> run set" ("\<lbrakk>\<lbrakk> _ \<rbrakk>\<rbrakk>\<^sub>s\<^sub>y\<^sub>m\<^sub>r\<^sub>u\<^sub>n") where
     "\<lbrakk>\<lbrakk> [] \<rbrakk>\<rbrakk>\<^sub>s\<^sub>y\<^sub>m\<^sub>r\<^sub>u\<^sub>n = { _. True }"
